Foundation/Modal/Logic/Sublogic/Grz.lean
@@ -21,7 +21,7 @@ instance : ProperSublogic Logic.S4 Logic.Grz := ⟨S4_ssubset_Grz⟩
 lemma Grz_ssubset_S5Grz : Logic.Grz ⊂ Logic.S5Grz := by
   constructor;
   . exact Hilbert.weakerThan_of_dominate_axioms (by simp) |>.subset;
-  . suffices ∃ φ, Hilbert.S5Grz ⊢! φ ∧ ¬FrameClass.finite_strict_preorder ⊧ φ by simpa [Grz.eq_ReflexiveTransitiveAntiSymmetricFiniteKripkeFrameClass_Logic];
+  . suffices ∃ φ, Hilbert.S5Grz ⊢! φ ∧ ¬FrameClass.finite_partial_order ⊧ φ by simpa [Grz.eq_ReflexiveTransitiveAntiSymmetricFiniteKripkeFrameClass_Logic];
     use Axioms.Five (.atom 0)
     constructor;
     . exact axiomFive!;
